\documentclass[11pt]{article}

\usepackage{kotex}
\usepackage{latexsym}
\usepackage{amssymb}
\usepackage{bm}

\newcommand{\sumnbr}{\sum_{\mbox{nbr}}}

\begin{document}
Hello Wolrd!

$y=2x-1$ 

\(y=2x-1\)

\begin{math}
y=2x-1
\end{math}

$$y=2x-1$$

$x^{2y}, x^{{2y}^x}, X_{n_1}^{2y^z}$ \\ \\

$X^{2m}_{3m}, X^2n_3m$ \\

$X^2_n, X_n^2, X_{n^2}$ \\

$2^{2^{2^{2^{2^{2^{2^{2}}}}}}}$ \\

$f'(x) \quad f'''(x)|_{x=0}$ \\

$\pi, \Phi, \Sigma, \mu, \alpha$ \\

${\mit \Gamma \Pi \Phi}$는 $\Gamma \Pi \Phi$와 다르다. \\

... $\mathit{\Psi \Theta \Omega}$는 $\Psi \Theta \Omega$와 다르다. \\

$\sqrt[n]{x}, \sqrt[3]{ax+b}, \sqrt[2]{5}, \sqrt{2}, \sqrt[x]
{2}$ \\

\begin{equation} \label{eq:sqrt}
\sqrt{1+\sqrt{1+\sqrt{1+\sqrt{1+\sqrt{1+\sqrt{1+x}}}}}}
\end{equation} \\

$$\sqrt{\mathstrut a} \sqrt{\mathstrut d} \sqrt{\mathstrut g}$$

$(x_1+\cdots+x_n)$

$(a_1, \ldots, a_m)$

$(a_1, \vdots, a_n)$

$(a_1, \ddots, a_n)$

$\displaystyle \frac{x^2+1}{y_1^2-1}$ \\

$\displaystyle 1+\frac{1}{1+\frac{1}{1+\frac{1}{1+\frac{1}{1+\frac{1}{1+x}}}}}$

$\frac12$ $\frac x2$

${\cal A} \otimes$

${\cal A} \unlhd$

${\cal S}$를 ${\cal S}=\{A \bigm| A \ni{\cal T}\}$라 하자.

$\not 1, \emptyset$

$\not\ni, \not\subset, \not<$

$\lim_{n\to\infty}$ \\

$\displaystyle \liminf_{n\longrightarrow \infty}$ \\

$\displaystyle liminf_{n\longrightarrow \infty}$ \\

$a \bmod b \qquad y \pmod{a+b}$

$\int \int \cdots \int f dP$

$\int \! \int \cdots \int f dP$

$\int \!\! \int \cdots \int f dP$

$1/ \! \log n$

$\sqrt{4} \, n$

\[
f(x;\mu,\sigma) = \frac{1}{\sqrt{2\pi}\sigma} \exp\Bigl\{-\frac{(x-\mu)^2}{2\sigma^2} \Bigr\}
\]

$f(x;\mu,\sigma) = \frac{1}{\sqrt{2\pi}\sigma} \exp\Bigl\{-\frac{(x-\mu)^2}{2\sigma^2} \Bigr\}$

$$\sum_{i=1}^n x_i = \int_0^1 f$$

$\sum_{i=1}^n x_i = \int_0^1 f$

$\displaystyle{\frac{a-b}{c+d}}$

$\frac{\displaystyle a-b}{\displaystyle c+d}$

$$\displaystyle \vec{x} + \vec{y} = \left\{\begin{array}{l} a \\ b \end{array}\right.$$

\[
\textbf{A} = \left(\begin{array}{ccc} a_{11}& a_{12}& a_{13}\\
a_{21}& a_{22}& a_{23}\\
a_{31}& a_{32}& a_{33}
\end{array} \right)
\]

$$\widehat{a-1} = \widetilde{x-y} + \widehat{\mbox{Cov}}$$

\[
\begin{array}{lrc}
a & b & c \\
a-b & b-c & c-a \\
x^2+2x+1 & x^2+2x+1 & x^2+2x+1
\end{array}
\]

\begin{equation}
\begin{array}{*{3}{c@{+}}c@{=}c}
a_{11}x_1 & a_{12}x_2 & \cdots & a_{1n}x_n & b_1 \\
a_{11}x_1 & a_{12}x_2 & \cdots & a_{1n}x_n & b_1 \\
\multicolumn{5}{c}{\vdots} \\
a_{11}x_1 & a_{12}x_2 & \cdots & a_{1n}x_n & b_1
\end{array}
\end{equation}

$\left( \begin{array}{c} 
\left| \begin{array}{cc} 
a & b \\
c & d
\end{array} \right| \\
e \\
f 
\end{array} \right) $

$$x^n = \overbrace{x\times x \times \cdots \times x}$$

$$\overbrace{a+\underbrace{b+\overline{c+d}}+e}$$

$$\overbrace{a+\underbrace{b+c}_{123}+e}^{ab}$$

\begin{equation} \label{eq:logodds}
\frac{p(x_i|\textbf{x}_{-i})}{1-p(x_i|\textbf{x}_{-i})} = \theta_1 \sum_{i=1}^m x_i + \beta_1 \sumnbr x_ix_{i'}
\end{equation} 

\begin{equation}
\frac{p(x_i|\bm{x}_{-i})}{1-p(x_i|\bm{x}_{-i})} = \theta_1 \sum_{i=1}^m x_i + \beta_1 \sumnbr x_ix_{i'}
\end{equation} 

Test the above equation label in here (\ref{eq:logodds}).

\begin{eqnarray}
(x+y)^2 & = & x^2 + xy + yx + y^2 \label{eqnarray1} \\
		& = & x^2 + xy + xy + y^2 \nonumber \\
		& = & x^2 + 2xy + y^2 \label{eqnarray2}
\end{eqnarray}

\begin{eqnarray}
(x+y)^2 & = & x^2 + xy + yx + y^2 \\
		& = & x^2 + 2xy + y^2 \nonumber
\end{eqnarray}

\begin{eqnarray*}
(x+y)^2 & = & x^2 + xy + yx + y^2 \\
		& = & x^2 + 2xy + y^2 \nonumber
\end{eqnarray*}

\begin{eqnarray*}
\lefteqn{a+b+c+d+e+f+g+h+i+j+k+l=} \\
& & x+y+z+a+b+c+d+e+f+g+o+s+t+ \\
& & u+v+w
\end{eqnarray*}




















\end{document}